remove Ipred relation

src/Prelude/Limits_and_Successors.v
@@ -7,44 +7,41 @@ Generalizable All Variables.
 (**
   [x] is an immediate predecessor of [y]
 *)
-Definition Least {A:Type}{lt : relation A}
+Definition Least `{lt : relation A}
            {sto : StrictOrder lt} (x : A):=
   forall y,  clos_refl A lt x y.
 
 
-Definition Ipred {A:Type}{lt : relation A}
-           {sto : StrictOrder lt} (x y : A):=
+Definition Successor `{lt : relation A}
+           {sto : StrictOrder lt} (y x : A):=
   lt x y /\ (forall z,  lt x z -> lt z y -> False).
-
-
-Definition Successor {A:Type}{lt : relation A}
-           {sto : StrictOrder lt} (y x : A):= Ipred x y.
 
 (* omega limit *)
 
-Definition  Omega_limit
-            {A:Type}{lt : relation A}
-           {sto : StrictOrder lt} (s: nat -> A) (x:A)  :=
-  (forall i: nat, lt (s i) x) /\
-  (forall y, lt y  x -> exists i:nat, lt y (s i)).
 
 
-Definition Limit   {A:Type}{lt : relation A}
+Definition Limit   `{lt : relation A}
            {sto : StrictOrder lt}  (x:A)  :=
   (exists w:A,  lt w x) /\
   (forall y:A, lt y x -> exists z:A, lt y z /\ lt z x).
 
+Definition  Omega_limit
+            `{lt : relation A}
+           {sto : StrictOrder lt} (s: nat -> A) (x:A)  :=
+  (forall i: nat, lt (s i) x) /\
+  (forall y, lt y  x -> exists i:nat, lt y (s i)).
+
 (* the same, with a [sig]-type *)
 
 Definition  Omega_limit_s
-              {A:Type}{lt : relation A}
+             `{lt : relation A}
               {sto : StrictOrder lt}
               (s: nat -> A) (x:A) : Type :=
   ((forall i: nat, lt (s i) x) *
   (forall y, lt y  x ->  {i:nat | lt y (s i)}))%type.
 
 
-Lemma Omega_limit_not_Succ  {A:Type}{lt : relation A}
+Lemma Omega_limit_not_Succ  `{lt : relation A}
       {sto : StrictOrder lt} (s: nat -> A) (x:A) :
   Omega_limit s x ->
   forall y,  ~ Successor x y.
@@ -56,7 +53,7 @@ Proof.
    + destruct (Hsucc0 _ Hi (Hlim i)).
 Qed.
 
-Lemma Omega_limit_Limit {A:Type}{lt : relation A}
+Lemma Omega_limit_Limit `{lt : relation A}
       {sto : StrictOrder lt} (s: nat -> A) (x:A) :
   Omega_limit s x -> Limit x.
 Proof.
