src/Prelude/Ordinal_generic.v
@@ -13,19 +13,15 @@ Generalizable All Variables.
 Class OrdinalNotation {A:Type}{lt: relation A}(sto:StrictOrder lt)
       (compare : A -> A -> comparison)  :=
   { compare_correct :
-
       forall alpha beta:A,
         CompareSpec (alpha=beta) (lt alpha beta) (lt beta alpha)
                     (compare alpha beta);
     wf : well_founded lt;
-    ZeroLimitSucc_dec : forall alpha,  {Least alpha}+
-                                   {Limit alpha} +
-                                   {beta: A | Successor alpha beta}
+    ZeroLimitSucc_dec : forall alpha,
+        {Least alpha}+
+        {Limit alpha} +
+        {beta: A | Successor alpha beta}
   }. 
-
-
-
-
 
 (** The segment called [O alpha] in Schutte *)
 
@@ -34,8 +30,6 @@ Definition bigO `{nA : @OrdinalNotation A ltA stoA compareA}
   fun x: A => ltA x a.
 
 
-
-           
 (** The segment associated with nA is isomorphic to
     the interval [0,b[ *)
 
